unit-tests/Tests_verit.v
@@ -147,6 +147,10 @@ Section Checker_Bv1.
   Verit_Checker "bv1.smt2" "bv1.log".
 End Checker_Bv1.
 
+Section Checker_Bv2.
+  Verit_Checker "bv2.smt2" "bv2.log".
+End Checker_Bv2.
+
 
 Section Sat0.
   Parse_certif_verit t_i0 t_func0 t_atom0 t_form0 root0 used_roots0 trace0 "sat0.smt2" "sat0.vtlog".
@@ -318,6 +322,11 @@ Section Bv1.
   Compute @Euf_Checker.checker t_i_bv1 t_func_bv1 t_atom_bv1 t_form_bv1 root_bv1 used_roots_bv1 trace_bv1.
 End Bv1.
 
+Section Bv2.
+  Parse_certif_verit t_i_bv2 t_func_bv2 t_atom_bv2 t_form_bv2 root_bv2 used_roots_bv2 trace_bv2 "bv2.smt2" "bv2.log".
+  Compute @Euf_Checker.checker t_i_bv2 t_func_bv2 t_atom_bv2 t_form_bv2 root_bv2 used_roots_bv2 trace_bv2.
+End Bv2.
+
 
 Section Theorem_Sat0.
   Time Verit_Theorem theorem_sat0 "sat0.smt2" "sat0.vtlog".
@@ -457,6 +466,10 @@ Check theorem_lia5_holes.
 Section Theorem_Bv1.
   Time Verit_Theorem theorem_bv1 "bv1.smt2" "bv1.log".
 End Theorem_Bv1.
+
+Section Theorem_Bv2.
+  Time Verit_Theorem theorem_bv2 "bv2.smt2" "bv2.log".
+End Theorem_Bv2.
 
 
 (* verit tactic *)
